GMLInit/Data/Pi.lean
@@ -5,7 +5,7 @@ import GMLInit.Meta.Basic
 
 namespace Function
 
-protected def equiv {α₁ α₂ β₁ β₂} (e : Equiv α₁ α₂) (f : Equiv β₁ β₂) : Equiv (α₁ → β₁) (α₂ → β₂) where
+def equiv {α₁ α₂ β₁ β₂} (e : Equiv α₁ α₂) (f : Equiv β₁ β₂) : Equiv (α₁ → β₁) (α₂ → β₂) where
   fwd h₁ := f.fwd ∘ h₁ ∘ e.rev
   rev h₂ := f.rev ∘ h₂ ∘ e.fwd
   spec h₁ h₂ := by
@@ -31,16 +31,16 @@ def equivFst {α₁ α₂} (β : α₁ → Sort _) (e : Equiv α₁ α₂) : Equ
   spec f₁ f₂ := by
     split
     · intro h
-      rw [←h]
+      cases h
       funext x₁
-      apply eqRec_eq_of_heq
-      simp only []
+      apply dcast_eq_of_heq_of_eq
+      clean
       rw [e.rev_fwd x₁]
       reflexivity using (.≅.)
     · intro h
-      rw [←h]
+      cases h
       funext x₂
-      apply eqRec_eq_of_heq
+      apply dcast_eq_of_heq_of_eq
       rw [e.fwd_rev x₂]
       reflexivity using (.≅.)
 
@@ -50,23 +50,21 @@ def equivSnd {α} {β₁ : α → Sort _} {β₂ : α → Sort _} (e : (x : α) 
   spec f₁ f₂ := by
     split
     · intro h
-      rw [←h]
+      cases h
       funext x
-      simp only []
+      clean
       rw [(e x).rev_fwd]
     · intro h
-      rw [←h]
+      cases h
       funext x
-      simp only []
+      clean
       rw [(e x).fwd_rev]
 
 protected def equiv {α₁ α₂} {β₁ : α₁ → Sort _} {β₂ : α₂ → Sort _} (e : Equiv α₁ α₂) (f : (x₁ : α₁) → Equiv (β₁ x₁) (β₂ (e.fwd x₁))) : Equiv ((x₁ : α₁) → β₁ x₁) ((x₂ : α₂) → β₂ x₂) :=
-  let h1 : Equiv ((x₁ : α₁) → β₁ x₁) ((x₂ : α₂) → β₁ (e.rev x₂))
-    := equivFst β₁ e
-  let h2 : Equiv ((x₂ : α₂) → β₁ (e.rev x₂)) ((x₂ : α₂) → β₂ (e.fwd (e.rev x₂)))
-    := equivSnd (λ x₂ => f (e.rev x₂))
-  Equiv.comp h (Equiv.comp h2 h1)
-  where h := {
+  Equiv.comp h3 (Equiv.comp h2 h1) where
+  h1 := equivFst β₁ e
+  h2 := equivSnd (λ x₂ => f (e.rev x₂))
+  h3 := {
     rev := λ m x => (e.fwd_rev x).symm ▸ m x
     fwd := λ n x => (e.fwd_rev x) ▸ n x
     spec := λ m n => by
@@ -74,13 +72,13 @@ protected def equiv {α₁ α₂} {β₁ : α₁ → Sort _} {β₂ : α₂ → 
       · intro h
         rw [←h]
         funext x
-        simp only [eqRec_trans]
-        rw [eqRec_refl]
+        simp only [dcast_trans]
+        rw [dcast_refl]
       · intro h
         rw [←h]
         funext x
-        simp only [eqRec_trans]
-        rw [eqRec_refl]
+        simp only [dcast_trans]
+        rw [dcast_refl]
   }
 
 end Pi
